Scratch/Polymath.lean
@@ -25,8 +25,14 @@ def Word.pow : Word → Nat → Word :=
   | 0 => []
   | Nat.succ m => w ++ (pow w m)
 
+def Word.conj: Word → Letter → Word
+  | w, l => [l] ++ w ++ [l⁻¹]
+
 instance : Pow Word Nat where
   pow w n := w.pow n
+
+instance: Pow Word Letter where
+  pow w l := w.conj l
 
 def splits(l : Letter) : Word → List (Word × Word) 
   | [] => []
@@ -46,5 +52,116 @@ partial def l : Word → Nat
 #eval l ([α, α, β, α!, β!])
 
 #eval l ([α, α, β, α!, β!]^2)
+
+structure ProvedSplit (l: Letter)(w : Word) where
+  fst : Word
+  snd: Word
+  proof : w = fst ++ [l] ++ snd 
+
+def ProvedSplit.head (x: Letter) (ys: Word) : ProvedSplit x (x :: ys) :=
+  ⟨[], ys, rfl⟩
+
+def ProvedSplit.prepend{l: Letter}{w : Word} (x: Letter) 
+        (ps: ProvedSplit l w) : ProvedSplit l (x :: w) :=
+      let newFst := x :: ps.fst
+      let newSnd := ps.snd
+      have newProof : x :: w = newFst ++ [l] ++ newSnd  := 
+        by
+          let prev : x :: w = x :: (ps.fst ++ [l] ++ ps.snd) 
+             := congrArg  (List.cons x) ps.proof
+          rw [prev] 
+          simp
+      ⟨newFst, newSnd, newProof⟩   
+
+
+theorem conj_split (x: Letter) (ys fst snd: Word) :
+          ys = fst ++ [x⁻¹] ++ snd → x :: ys = fst^x ++ snd :=
+            by
+              intro hyp
+              have expand : fst^x = [x] ++ fst ++ [x⁻¹] := rfl
+              rw [expand] 
+              have lemma := 
+                    congrArg (List.cons x) hyp
+              rw [hyp]
+              simp
+
+abbrev Length := Word → Nat
+
+def conjInv(l: Length) : Prop := 
+    (x : Letter) → (g : Word) → l (g^x) = l (g)
+
+def triangIneq(l: Length) : Prop := 
+    (g h : Word) → l (g ++ h) ≤ l g + l h
+
+def normalized(l: Length) : Prop :=
+    (x : Letter) → l [x] = 1
+
+structure ProvedBound(g: Word):  Type where
+  bound: Nat 
+  pf : (l: Length) → normalized l → conjInv l → triangIneq l → l g ≤ bound
+
+def conjBound(x: Letter)(ys fst snd: Word)(eqn : ys = fst ++ [x⁻¹] ++ snd) :
+        ProvedBound fst → ProvedBound snd → ProvedBound (x :: ys) := 
+          fun pb1 pb2 =>
+          let bound := pb1.bound + pb2.bound
+          let pf : 
+            (l: Length) → normalized l → conjInv l → triangIneq l → 
+                l (x :: ys) ≤ bound := by
+                  intros l norm conj triang
+                  rw [conj_split x ys fst snd eqn]
+                  have lem : l (fst ^ x ++ snd) ≤ l (fst^x) + l snd := 
+                     by
+                       apply triang
+                  skip
+                  have clem : l (fst^x) = l fst := by apply conj
+                  rw [clem] at lem
+                  apply Nat.le_trans lem
+                  have l1 : l fst ≤ pb1.bound := pb1.pf l norm conj triang
+                  have l2 : l snd ≤ pb2.bound := pb2.pf l norm conj triang
+                  apply Nat.add_le_add l1 l2
+          ⟨bound, pf⟩
+
+def ProvedBound.prepend{w : Word} (x: Letter) 
+        (ps: ProvedBound w) : ProvedBound (x :: w) :=
+      let newBound := ps.bound + 1
+      ⟨newBound, fun l norm conj triang => by
+        let prev := ps.pf l norm conj triang
+        have lemTri : l (x :: w) ≤ l ([x]) + l w := 
+          by
+            apply triang [x] 
+        skip
+        apply Nat.le_trans lemTri
+        have gen : l [x] = 1 := norm x
+        rw [gen]
+        rw [Nat.add_comm]
+        apply Nat.add_le_add_right prev  
+        ⟩
+
+def ProvedBound.min {w: Word}: ProvedBound w → List (ProvedBound w) → 
+    ProvedBound w :=
+        fun head tail =>
+          tail.foldl (fun pb1 pb2 =>
+            if pb1.bound ≤ pb2.bound then pb1 else pb2) head
+
+def ProvedBound.empty: ProvedBound [] :=
+  ⟨0, sorry⟩
+
+
+def provedSplits(z: Letter) : (w : Word) → List (ProvedSplit z w) 
+  | [] => []
+  | x :: ys =>
+    let tailSplits := (provedSplits z ys).map (
+        fun ps => ps.prepend x) 
+    if c:x = z then
+      let headSplit : ProvedSplit z (x :: ys) :=
+        by
+          rw [c] 
+          exact ProvedSplit.head z ys 
+      headSplit :: tailSplits
+    else tailSplits
+
+#eval (provedSplits α [β, α, β, α, β⁻¹]).map (fun ps => (ps.fst, ps.snd))
+
+#check Nat.add_le_add_right
 
 end PolyMath
