Scratch/CzSlOly.lean
@@ -22,3 +22,4 @@ theorem CzSlOly : (∀ a b : M, (a * b) * b = a) → (∀ a b : M, a * (a * b) =
 example : (∀ a b : M, (a * b) * b = a) → (∀ a b : M, a * (a * b) = b) →
             (m n : M) →  (m * n) * n = m := by
             introsRwFind 2
+   
